backends/lean/Aeneas/Progress.lean
@@ -1,3 +1,4 @@
+import Aeneas.Progress.InferPost
 import Aeneas.Progress.Progress
 import Aeneas.Progress.ProgressArraySpec
 import Aeneas.Progress.ProgressStar
